added a bunch of lemmas in utils; proved with new definitions that unzip preserves abr and content of tree, up to the case where k appears in t

proofs/definitions.v
@@ -3,6 +3,7 @@ Require Export Lia.
 Require Export Coq.Sorting.Sorted.
 Require Export stdpp.sorting.
 From Equations Require Export Equations.
+From Coq.Program Require Export Equality.
 Global Open Scope bool_scope.
 
 Definition A := nat.
@@ -10,6 +11,8 @@ Definition A := nat.
 Parameter rank_of : A -> nat.
 
 Inductive Tree : Type := Leaf: Tree | Node: Tree -> A -> nat -> Tree -> Tree.
+
+Definition singleton (k: A) (r: nat) : Tree := Node Leaf k r Leaf.
 
 Equations elements (t: Tree) : list A :=
   elements Leaf := [];
@@ -20,9 +23,21 @@ Definition occurs (x: A) (t: Tree) := x ∈ elements t.
 Notation "x '∈' t" := (occurs x t).
 Notation "x '∉' t" := (~(occurs x t)).
 
-Definition all_smallers (t: Tree) (x: A) := forall y, y ∈ t -> y < x.
+Definition delta {X} (b: bool) (x: X) := if b then [x] else [].
 
-Definition all_greaters (t: Tree) (x: A) := forall y, y ∈ t -> x < y.
+Equations occursb_list (x: A) (l: list A) : bool :=
+| x, [] => false;
+| x, a::l0 with (x =? a), occursb_list x l0 => {
+  | true, _ => true;
+  | _, true => true;
+  | false, false => false;
+  }.
+
+Definition occursb (x: A) (t: Tree) := occursb_list x (elements t).
+
+Definition all_smallers (t: Tree) (x: A) := Forall (gt x) (elements t).
+
+Definition all_greaters (t: Tree) (x: A) := Forall (lt x) (elements t).
 
 Notation sorted := (StronglySorted lt).
 
